examples/Employee_DesignModel_UMLPart.thy
@@ -239,22 +239,22 @@ lemmas [simp] =
 
 subsection{* Context Passing *}
 
-lemma cp_OclAsType\<^sub>O\<^sub>c\<^sub>l\<^sub>A\<^sub>n\<^sub>y_Person_Person: "cp P \<Longrightarrow> cp(\<lambda>X. (P (X::Person) :: Person) .oclAsType(OclAny))"
+lemma cp_OclAsType\<^sub>O\<^sub>c\<^sub>l\<^sub>A\<^sub>n\<^sub>y_Person_Person: "cp P \<Longrightarrow> cp(\<lambda>X. (P (X::Person)::Person) .oclAsType(OclAny))"
 by(rule cpI1, simp_all add: OclAsType\<^sub>O\<^sub>c\<^sub>l\<^sub>A\<^sub>n\<^sub>y_Person)
-lemma cp_OclAsType\<^sub>O\<^sub>c\<^sub>l\<^sub>A\<^sub>n\<^sub>y_OclAny_OclAny: "cp P \<Longrightarrow> cp(\<lambda>X. (P (X::OclAny) :: OclAny) .oclAsType(OclAny))"
+lemma cp_OclAsType\<^sub>O\<^sub>c\<^sub>l\<^sub>A\<^sub>n\<^sub>y_OclAny_OclAny: "cp P \<Longrightarrow> cp(\<lambda>X. (P (X::OclAny)::OclAny) .oclAsType(OclAny))"
 by(rule cpI1, simp_all add: OclAsType\<^sub>O\<^sub>c\<^sub>l\<^sub>A\<^sub>n\<^sub>y_OclAny)
-lemma cp_OclAsType\<^sub>P\<^sub>e\<^sub>r\<^sub>s\<^sub>o\<^sub>n_Person_Person: "cp P \<Longrightarrow> cp(\<lambda>X. (P (X::Person) :: Person) .oclAsType(Person))"
+lemma cp_OclAsType\<^sub>P\<^sub>e\<^sub>r\<^sub>s\<^sub>o\<^sub>n_Person_Person: "cp P \<Longrightarrow> cp(\<lambda>X. (P (X::Person)::Person) .oclAsType(Person))"
 by(rule cpI1, simp_all add: OclAsType\<^sub>P\<^sub>e\<^sub>r\<^sub>s\<^sub>o\<^sub>n_Person)
-lemma cp_OclAsType\<^sub>P\<^sub>e\<^sub>r\<^sub>s\<^sub>o\<^sub>n_OclAny_OclAny: "cp P \<Longrightarrow> cp(\<lambda>X. (P (X::OclAny) :: OclAny) .oclAsType(Person))"
+lemma cp_OclAsType\<^sub>P\<^sub>e\<^sub>r\<^sub>s\<^sub>o\<^sub>n_OclAny_OclAny: "cp P \<Longrightarrow> cp(\<lambda>X. (P (X::OclAny)::OclAny) .oclAsType(Person))"
 by(rule cpI1, simp_all add: OclAsType\<^sub>P\<^sub>e\<^sub>r\<^sub>s\<^sub>o\<^sub>n_OclAny)
 
-lemma cp_OclAsType\<^sub>O\<^sub>c\<^sub>l\<^sub>A\<^sub>n\<^sub>y_Person_OclAny: "cp P \<Longrightarrow> cp(\<lambda>X. (P (X::Person) :: OclAny) .oclAsType(OclAny))"
+lemma cp_OclAsType\<^sub>O\<^sub>c\<^sub>l\<^sub>A\<^sub>n\<^sub>y_Person_OclAny: "cp P \<Longrightarrow> cp(\<lambda>X. (P (X::Person)::OclAny) .oclAsType(OclAny))"
 by(rule cpI1, simp_all add: OclAsType\<^sub>O\<^sub>c\<^sub>l\<^sub>A\<^sub>n\<^sub>y_OclAny)
-lemma cp_OclAsType\<^sub>O\<^sub>c\<^sub>l\<^sub>A\<^sub>n\<^sub>y_OclAny_Person: "cp P \<Longrightarrow> cp(\<lambda>X. (P (X::OclAny) :: Person) .oclAsType(OclAny))"
+lemma cp_OclAsType\<^sub>O\<^sub>c\<^sub>l\<^sub>A\<^sub>n\<^sub>y_OclAny_Person: "cp P \<Longrightarrow> cp(\<lambda>X. (P (X::OclAny)::Person) .oclAsType(OclAny))"
 by(rule cpI1, simp_all add: OclAsType\<^sub>O\<^sub>c\<^sub>l\<^sub>A\<^sub>n\<^sub>y_Person)
-lemma cp_OclAsType\<^sub>P\<^sub>e\<^sub>r\<^sub>s\<^sub>o\<^sub>n_Person_OclAny: "cp P \<Longrightarrow> cp(\<lambda>X. (P (X::Person) :: OclAny) .oclAsType(Person))"
+lemma cp_OclAsType\<^sub>P\<^sub>e\<^sub>r\<^sub>s\<^sub>o\<^sub>n_Person_OclAny: "cp P \<Longrightarrow> cp(\<lambda>X. (P (X::Person)::OclAny) .oclAsType(Person))"
 by(rule cpI1, simp_all add: OclAsType\<^sub>P\<^sub>e\<^sub>r\<^sub>s\<^sub>o\<^sub>n_OclAny)
-lemma cp_OclAsType\<^sub>P\<^sub>e\<^sub>r\<^sub>s\<^sub>o\<^sub>n_OclAny_Person: "cp P \<Longrightarrow> cp(\<lambda>X. (P (X::OclAny) :: Person) .oclAsType(Person))"
+lemma cp_OclAsType\<^sub>P\<^sub>e\<^sub>r\<^sub>s\<^sub>o\<^sub>n_OclAny_Person: "cp P \<Longrightarrow> cp(\<lambda>X. (P (X::OclAny)::Person) .oclAsType(Person))"
 by(rule cpI1, simp_all add: OclAsType\<^sub>P\<^sub>e\<^sub>r\<^sub>s\<^sub>o\<^sub>n_Person)
 
 lemmas [simp] =
@@ -335,23 +335,23 @@ defs (overloaded) OclIsTypeOf\<^sub>P\<^sub>e\<^sub>r\<^sub>s\<^sub>o\<^sub>n_Pe
 
 subsection{* Context Passing *}
 
-lemma cp_OclIsTypeOf\<^sub>O\<^sub>c\<^sub>l\<^sub>A\<^sub>n\<^sub>y_Person_Person: "cp P \<Longrightarrow> cp(\<lambda>X. (P (X::Person) :: Person) .oclIsTypeOf(OclAny))"
+lemma cp_OclIsTypeOf\<^sub>O\<^sub>c\<^sub>l\<^sub>A\<^sub>n\<^sub>y_Person_Person: "cp P \<Longrightarrow> cp(\<lambda>X.(P(X::Person)::Person).oclIsTypeOf(OclAny))"
 by(rule cpI1, simp_all add: OclIsTypeOf\<^sub>O\<^sub>c\<^sub>l\<^sub>A\<^sub>n\<^sub>y_Person)
-lemma cp_OclIsTypeOf\<^sub>O\<^sub>c\<^sub>l\<^sub>A\<^sub>n\<^sub>y_OclAny_OclAny: "cp P \<Longrightarrow> cp(\<lambda>X. (P (X::OclAny) :: OclAny) .oclIsTypeOf(OclAny))"
+lemma cp_OclIsTypeOf\<^sub>O\<^sub>c\<^sub>l\<^sub>A\<^sub>n\<^sub>y_OclAny_OclAny: "cp P \<Longrightarrow> cp(\<lambda>X.(P(X::OclAny)::OclAny).oclIsTypeOf(OclAny))"
 by(rule cpI1, simp_all add: OclIsTypeOf\<^sub>O\<^sub>c\<^sub>l\<^sub>A\<^sub>n\<^sub>y_OclAny)
-lemma cp_OclIsTypeOf\<^sub>P\<^sub>e\<^sub>r\<^sub>s\<^sub>o\<^sub>n_Person_Person: "cp P \<Longrightarrow> cp(\<lambda>X. (P (X::Person) :: Person) .oclIsTypeOf(Person))"
+lemma cp_OclIsTypeOf\<^sub>P\<^sub>e\<^sub>r\<^sub>s\<^sub>o\<^sub>n_Person_Person: "cp P \<Longrightarrow> cp(\<lambda>X.(P(X::Person)::Person).oclIsTypeOf(Person))"
 by(rule cpI1, simp_all add: OclIsTypeOf\<^sub>P\<^sub>e\<^sub>r\<^sub>s\<^sub>o\<^sub>n_Person)
-lemma cp_OclIsTypeOf\<^sub>P\<^sub>e\<^sub>r\<^sub>s\<^sub>o\<^sub>n_OclAny_OclAny: "cp P \<Longrightarrow> cp(\<lambda>X. (P (X::OclAny) :: OclAny) .oclIsTypeOf(Person))"
+lemma cp_OclIsTypeOf\<^sub>P\<^sub>e\<^sub>r\<^sub>s\<^sub>o\<^sub>n_OclAny_OclAny: "cp P \<Longrightarrow> cp(\<lambda>X.(P(X::OclAny)::OclAny).oclIsTypeOf(Person))"
 by(rule cpI1, simp_all add: OclIsTypeOf\<^sub>P\<^sub>e\<^sub>r\<^sub>s\<^sub>o\<^sub>n_OclAny)
 
 
-lemma cp_OclIsTypeOf\<^sub>O\<^sub>c\<^sub>l\<^sub>A\<^sub>n\<^sub>y_Person_OclAny: "cp P \<Longrightarrow> cp(\<lambda>X. (P (X::Person) :: OclAny) .oclIsTypeOf(OclAny))"
+lemma cp_OclIsTypeOf\<^sub>O\<^sub>c\<^sub>l\<^sub>A\<^sub>n\<^sub>y_Person_OclAny: "cp P \<Longrightarrow> cp(\<lambda>X.(P(X::Person)::OclAny).oclIsTypeOf(OclAny))"
 by(rule cpI1, simp_all add: OclIsTypeOf\<^sub>O\<^sub>c\<^sub>l\<^sub>A\<^sub>n\<^sub>y_OclAny)
-lemma cp_OclIsTypeOf\<^sub>O\<^sub>c\<^sub>l\<^sub>A\<^sub>n\<^sub>y_OclAny_Person: "cp P \<Longrightarrow> cp(\<lambda>X. (P (X::OclAny) :: Person) .oclIsTypeOf(OclAny))"
+lemma cp_OclIsTypeOf\<^sub>O\<^sub>c\<^sub>l\<^sub>A\<^sub>n\<^sub>y_OclAny_Person: "cp P \<Longrightarrow> cp(\<lambda>X.(P(X::OclAny)::Person).oclIsTypeOf(OclAny))"
 by(rule cpI1, simp_all add: OclIsTypeOf\<^sub>O\<^sub>c\<^sub>l\<^sub>A\<^sub>n\<^sub>y_Person)
-lemma cp_OclIsTypeOf\<^sub>P\<^sub>e\<^sub>r\<^sub>s\<^sub>o\<^sub>n_Person_OclAny: "cp P \<Longrightarrow> cp(\<lambda>X. (P (X::Person) :: OclAny) .oclIsTypeOf(Person))"
+lemma cp_OclIsTypeOf\<^sub>P\<^sub>e\<^sub>r\<^sub>s\<^sub>o\<^sub>n_Person_OclAny: "cp P \<Longrightarrow> cp(\<lambda>X.(P(X::Person)::OclAny).oclIsTypeOf(Person))"
 by(rule cpI1, simp_all add: OclIsTypeOf\<^sub>P\<^sub>e\<^sub>r\<^sub>s\<^sub>o\<^sub>n_OclAny)
-lemma cp_OclIsTypeOf\<^sub>P\<^sub>e\<^sub>r\<^sub>s\<^sub>o\<^sub>n_OclAny_Person: "cp P \<Longrightarrow> cp(\<lambda>X. (P (X::OclAny) :: Person) .oclIsTypeOf(Person))"
+lemma cp_OclIsTypeOf\<^sub>P\<^sub>e\<^sub>r\<^sub>s\<^sub>o\<^sub>n_OclAny_Person: "cp P \<Longrightarrow> cp(\<lambda>X.(P(X::OclAny)::Person).oclIsTypeOf(Person))"
 by(rule cpI1, simp_all add: OclIsTypeOf\<^sub>P\<^sub>e\<^sub>r\<^sub>s\<^sub>o\<^sub>n_Person)
 
 lemmas [simp] =
@@ -493,22 +493,22 @@ defs (overloaded) OclIsKindOf\<^sub>P\<^sub>e\<^sub>r\<^sub>s\<^sub>o\<^sub>n_Pe
 
 subsection{* Context Passing *}
 
-lemma cp_OclIsKindOf\<^sub>O\<^sub>c\<^sub>l\<^sub>A\<^sub>n\<^sub>y_Person_Person: "cp P \<Longrightarrow> cp(\<lambda>X. (P (X::Person) :: Person) .oclIsKindOf(OclAny))"
+lemma cp_OclIsKindOf\<^sub>O\<^sub>c\<^sub>l\<^sub>A\<^sub>n\<^sub>y_Person_Person: "cp P \<Longrightarrow> cp(\<lambda>X.(P(X::Person)::Person).oclIsKindOf(OclAny))"
 by(rule cpI1, simp_all add: OclIsKindOf\<^sub>O\<^sub>c\<^sub>l\<^sub>A\<^sub>n\<^sub>y_Person)
-lemma cp_OclIsKindOf\<^sub>O\<^sub>c\<^sub>l\<^sub>A\<^sub>n\<^sub>y_OclAny_OclAny: "cp P \<Longrightarrow> cp(\<lambda>X. (P (X::OclAny) :: OclAny) .oclIsKindOf(OclAny))"
+lemma cp_OclIsKindOf\<^sub>O\<^sub>c\<^sub>l\<^sub>A\<^sub>n\<^sub>y_OclAny_OclAny: "cp P \<Longrightarrow> cp(\<lambda>X.(P(X::OclAny)::OclAny).oclIsKindOf(OclAny))"
 by(rule cpI1, simp_all add: OclIsKindOf\<^sub>O\<^sub>c\<^sub>l\<^sub>A\<^sub>n\<^sub>y_OclAny)
-lemma cp_OclIsKindOf\<^sub>P\<^sub>e\<^sub>r\<^sub>s\<^sub>o\<^sub>n_Person_Person: "cp P \<Longrightarrow> cp(\<lambda>X. (P (X::Person) :: Person) .oclIsKindOf(Person))"
+lemma cp_OclIsKindOf\<^sub>P\<^sub>e\<^sub>r\<^sub>s\<^sub>o\<^sub>n_Person_Person: "cp P \<Longrightarrow> cp(\<lambda>X.(P(X::Person)::Person).oclIsKindOf(Person))"
 by(rule cpI1, simp_all add: OclIsKindOf\<^sub>P\<^sub>e\<^sub>r\<^sub>s\<^sub>o\<^sub>n_Person)
-lemma cp_OclIsKindOf\<^sub>P\<^sub>e\<^sub>r\<^sub>s\<^sub>o\<^sub>n_OclAny_OclAny: "cp P \<Longrightarrow> cp(\<lambda>X. (P (X::OclAny) :: OclAny) .oclIsKindOf(Person))"
+lemma cp_OclIsKindOf\<^sub>P\<^sub>e\<^sub>r\<^sub>s\<^sub>o\<^sub>n_OclAny_OclAny: "cp P \<Longrightarrow> cp(\<lambda>X.(P(X::OclAny)::OclAny).oclIsKindOf(Person))"
 by(rule cpI1, simp_all add: OclIsKindOf\<^sub>P\<^sub>e\<^sub>r\<^sub>s\<^sub>o\<^sub>n_OclAny)
 
-lemma cp_OclIsKindOf\<^sub>O\<^sub>c\<^sub>l\<^sub>A\<^sub>n\<^sub>y_Person_OclAny: "cp P \<Longrightarrow> cp(\<lambda>X. (P (X::Person) :: OclAny) .oclIsKindOf(OclAny))"
+lemma cp_OclIsKindOf\<^sub>O\<^sub>c\<^sub>l\<^sub>A\<^sub>n\<^sub>y_Person_OclAny: "cp P \<Longrightarrow> cp(\<lambda>X.(P(X::Person)::OclAny).oclIsKindOf(OclAny))"
 by(rule cpI1, simp_all add: OclIsKindOf\<^sub>O\<^sub>c\<^sub>l\<^sub>A\<^sub>n\<^sub>y_OclAny)
-lemma cp_OclIsKindOf\<^sub>O\<^sub>c\<^sub>l\<^sub>A\<^sub>n\<^sub>y_OclAny_Person: "cp P \<Longrightarrow> cp(\<lambda>X. (P (X::OclAny) :: Person) .oclIsKindOf(OclAny))"
+lemma cp_OclIsKindOf\<^sub>O\<^sub>c\<^sub>l\<^sub>A\<^sub>n\<^sub>y_OclAny_Person: "cp P \<Longrightarrow> cp(\<lambda>X.(P(X::OclAny)::Person).oclIsKindOf(OclAny))"
 by(rule cpI1, simp_all add: OclIsKindOf\<^sub>O\<^sub>c\<^sub>l\<^sub>A\<^sub>n\<^sub>y_Person)
-lemma cp_OclIsKindOf\<^sub>P\<^sub>e\<^sub>r\<^sub>s\<^sub>o\<^sub>n_Person_OclAny: "cp P \<Longrightarrow> cp(\<lambda>X. (P (X::Person) :: OclAny) .oclIsKindOf(Person))"
+lemma cp_OclIsKindOf\<^sub>P\<^sub>e\<^sub>r\<^sub>s\<^sub>o\<^sub>n_Person_OclAny: "cp P \<Longrightarrow> cp(\<lambda>X.(P(X::Person)::OclAny).oclIsKindOf(Person))"
 by(rule cpI1, simp_all add: OclIsKindOf\<^sub>P\<^sub>e\<^sub>r\<^sub>s\<^sub>o\<^sub>n_OclAny)
-lemma cp_OclIsKindOf\<^sub>P\<^sub>e\<^sub>r\<^sub>s\<^sub>o\<^sub>n_OclAny_Person: "cp P \<Longrightarrow> cp(\<lambda>X. (P (X::OclAny) :: Person) .oclIsKindOf(Person))"
+lemma cp_OclIsKindOf\<^sub>P\<^sub>e\<^sub>r\<^sub>s\<^sub>o\<^sub>n_OclAny_Person: "cp P \<Longrightarrow> cp(\<lambda>X.(P(X::OclAny)::Person).oclIsKindOf(Person))"
 by(rule cpI1, simp_all add: OclIsKindOf\<^sub>P\<^sub>e\<^sub>r\<^sub>s\<^sub>o\<^sub>n_Person)
 
 lemmas [simp] =
@@ -588,7 +588,8 @@ lemmas [simp] = Person_def OclAny_def
 lemma OclAllInstances_generic\<^sub>O\<^sub>c\<^sub>l\<^sub>A\<^sub>n\<^sub>y_exec: "OclAllInstances_generic pre_post OclAny =
              (\<lambda>\<tau>.  Abs_Set_0  \<lfloor>\<lfloor> Some ` OclAny ` ran (heap (pre_post \<tau>)) \<rfloor>\<rfloor>)"
  apply(rule ext, simp add: OclAllInstances_generic_def)
- apply(subgoal_tac " (OclAny ` ran (heap (pre_post \<tau>)) - {None}) = (OclAny ` ran (heap (pre_post \<tau>)))", simp)
+ apply(subgoal_tac "OclAny ` ran (heap (pre_post \<tau>)) - {None} = OclAny ` ran (heap (pre_post \<tau>))",
+       simp)
  apply(simp add: image_def)
  apply(rule equalityI)
  apply(rule subsetI)
@@ -616,7 +617,8 @@ lemma OclAny_allInstances_generic_oclIsTypeOf\<^sub>O\<^sub>c\<^sub>l\<^sub>A\<^
 assumes [simp]: "\<And>x. pre_post (x, x) = x"
 shows "\<exists>\<tau>. (\<tau> \<Turnstile>     ((OclAllInstances_generic pre_post OclAny)->forAll(X|X .oclIsTypeOf(OclAny))))"
  apply(rule_tac x = \<tau>\<^sub>0 in exI, simp add: \<tau>\<^sub>0_def OclValid_def del: OclAllInstances_generic_def)
- apply(simp only: assms OclForall_def OclAllInstances_generic_defined[simplified OclValid_def] refl if_True)
+ apply(simp only: assms OclForall_def refl if_True
+                  OclAllInstances_generic_defined[simplified OclValid_def])
  apply(simp only: OclAllInstances_generic_def)
  apply(subst (1 2 3) Abs_Set_0_inverse, simp add: bot_option_def)
 by(simp add: OclIsTypeOf\<^sub>O\<^sub>c\<^sub>l\<^sub>A\<^sub>n\<^sub>y_OclAny)
@@ -637,7 +639,8 @@ shows "\<exists>\<tau>. (\<tau> \<Turnstile> not ((OclAllInstances_generic pre_p
 proof - fix oid a let ?t0 = "\<lparr>heap = empty(oid \<mapsto> in\<^sub>O\<^sub>c\<^sub>l\<^sub>A\<^sub>n\<^sub>y (mk\<^sub>O\<^sub>c\<^sub>l\<^sub>A\<^sub>n\<^sub>y oid \<lfloor>a\<rfloor>)),
                               assocs\<^sub>2 = empty, assocs\<^sub>3 = empty\<rparr>" show ?thesis
  apply(rule_tac x = "(?t0, ?t0)" in exI, simp add: OclValid_def del: OclAllInstances_generic_def)
- apply(simp only: OclForall_def OclAllInstances_generic_defined[simplified OclValid_def] refl if_True)
+ apply(simp only: OclForall_def refl if_True
+                  OclAllInstances_generic_defined[simplified OclValid_def])
  apply(simp only: OclAllInstances_generic_def OclAsType\<^sub>O\<^sub>c\<^sub>l\<^sub>A\<^sub>n\<^sub>y_\<AA>_def)
  apply(subst (1 2 3) Abs_Set_0_inverse, simp add: bot_option_def)
  by(simp add: OclIsTypeOf\<^sub>O\<^sub>c\<^sub>l\<^sub>A\<^sub>n\<^sub>y_OclAny OclNot_def OclAny_def)
@@ -656,7 +659,8 @@ by(rule OclAny_allInstances_generic_oclIsTypeOf\<^sub>O\<^sub>c\<^sub>l\<^sub>A\
 lemma Person_allInstances_generic_oclIsTypeOf\<^sub>P\<^sub>e\<^sub>r\<^sub>s\<^sub>o\<^sub>n:
 "\<tau> \<Turnstile> ((OclAllInstances_generic pre_post Person)->forAll(X|X .oclIsTypeOf(Person)))"
  apply(simp add: OclValid_def del: OclAllInstances_generic_def)
- apply(simp only: OclForall_def OclAllInstances_generic_defined[simplified OclValid_def] refl if_True)
+ apply(simp only: OclForall_def refl if_True
+                  OclAllInstances_generic_defined[simplified OclValid_def])
  apply(simp only: OclAllInstances_generic_def)
  apply(subst (1 2 3) Abs_Set_0_inverse, simp add: bot_option_def)
 by(simp add: OclIsTypeOf\<^sub>P\<^sub>e\<^sub>r\<^sub>s\<^sub>o\<^sub>n_Person)
@@ -675,7 +679,8 @@ subsection{* OclIsKindOf *}
 lemma OclAny_allInstances_generic_oclIsKindOf\<^sub>O\<^sub>c\<^sub>l\<^sub>A\<^sub>n\<^sub>y:
 "\<tau> \<Turnstile> ((OclAllInstances_generic pre_post OclAny)->forAll(X|X .oclIsKindOf(OclAny)))"
  apply(simp add: OclValid_def del: OclAllInstances_generic_def)
- apply(simp only: OclForall_def OclAllInstances_generic_defined[simplified OclValid_def] refl if_True)
+ apply(simp only: OclForall_def refl if_True
+                  OclAllInstances_generic_defined[simplified OclValid_def])
  apply(simp only: OclAllInstances_generic_def)
  apply(subst (1 2 3) Abs_Set_0_inverse, simp add: bot_option_def)
 by(simp add: OclIsKindOf\<^sub>O\<^sub>c\<^sub>l\<^sub>A\<^sub>n\<^sub>y_OclAny)
@@ -693,7 +698,8 @@ by(rule OclAny_allInstances_generic_oclIsKindOf\<^sub>O\<^sub>c\<^sub>l\<^sub>A\
 lemma Person_allInstances_generic_oclIsKindOf\<^sub>O\<^sub>c\<^sub>l\<^sub>A\<^sub>n\<^sub>y:
 "\<tau> \<Turnstile> ((OclAllInstances_generic pre_post Person)->forAll(X|X .oclIsKindOf(OclAny)))"
  apply(simp add: OclValid_def del: OclAllInstances_generic_def)
- apply(simp only: OclForall_def OclAllInstances_generic_defined[simplified OclValid_def] refl if_True)
+ apply(simp only: OclForall_def refl if_True
+                  OclAllInstances_generic_defined[simplified OclValid_def])
  apply(simp only: OclAllInstances_generic_def)
  apply(subst (1 2 3) Abs_Set_0_inverse, simp add: bot_option_def)
 by(simp add: OclIsKindOf\<^sub>O\<^sub>c\<^sub>l\<^sub>A\<^sub>n\<^sub>y_Person)
@@ -711,7 +717,8 @@ by(rule Person_allInstances_generic_oclIsKindOf\<^sub>O\<^sub>c\<^sub>l\<^sub>A\
 lemma Person_allInstances_generic_oclIsKindOf\<^sub>P\<^sub>e\<^sub>r\<^sub>s\<^sub>o\<^sub>n:
 "\<tau> \<Turnstile> ((OclAllInstances_generic pre_post Person)->forAll(X|X .oclIsKindOf(Person)))"
  apply(simp add: OclValid_def del: OclAllInstances_generic_def)
- apply(simp only: OclForall_def OclAllInstances_generic_defined[simplified OclValid_def] refl if_True)
+ apply(simp only: OclForall_def refl if_True
+                  OclAllInstances_generic_defined[simplified OclValid_def])
  apply(simp only: OclAllInstances_generic_def)
  apply(subst (1 2 3) Abs_Set_0_inverse, simp add: bot_option_def)
 by(simp add: OclIsKindOf\<^sub>P\<^sub>e\<^sub>r\<^sub>s\<^sub>o\<^sub>n_Person)
@@ -819,13 +826,15 @@ lemmas [simp] =
 
 subsection{* Context Passing *}
 
-lemma cp_dot\<^sub>O\<^sub>c\<^sub>l\<^sub>A\<^sub>n\<^sub>y\<A>\<N>\<Y>: "((X).any) \<tau> = ((\<lambda>_. X \<tau>).any) \<tau>" by(simp add: eval_extract_def)
-lemma cp_dot\<^sub>P\<^sub>e\<^sub>r\<^sub>s\<^sub>o\<^sub>n\<B>\<O>\<S>\<S>: "((X).boss) \<tau> = ((\<lambda>_. X \<tau>).boss) \<tau>" by(simp add: eval_extract_def)
-lemma cp_dot\<^sub>P\<^sub>e\<^sub>r\<^sub>s\<^sub>o\<^sub>n\<S>\<A>\<L>\<A>\<R>\<Y>: "((X).salary) \<tau> = ((\<lambda>_. X \<tau>).salary) \<tau>" by(simp add: eval_extract_def)
+lemmas [simp] = eval_extract_def
 
-lemma cp_dot\<^sub>O\<^sub>c\<^sub>l\<^sub>A\<^sub>n\<^sub>y\<A>\<N>\<Y>_at_pre: "((X).any@pre) \<tau> = ((\<lambda>_. X \<tau>).any@pre) \<tau>" by(simp add: eval_extract_def)
-lemma cp_dot\<^sub>P\<^sub>e\<^sub>r\<^sub>s\<^sub>o\<^sub>n\<B>\<O>\<S>\<S>_at_pre: "((X).boss@pre) \<tau> = ((\<lambda>_. X \<tau>).boss@pre) \<tau>" by(simp add: eval_extract_def)
-lemma cp_dot\<^sub>P\<^sub>e\<^sub>r\<^sub>s\<^sub>o\<^sub>n\<S>\<A>\<L>\<A>\<R>\<Y>_at_pre: "((X).salary@pre) \<tau> = ((\<lambda>_. X \<tau>).salary@pre) \<tau>" by(simp add: eval_extract_def)
+lemma cp_dot\<^sub>O\<^sub>c\<^sub>l\<^sub>A\<^sub>n\<^sub>y\<A>\<N>\<Y>: "((X).any) \<tau> = ((\<lambda>_. X \<tau>).any) \<tau>" by simp
+lemma cp_dot\<^sub>P\<^sub>e\<^sub>r\<^sub>s\<^sub>o\<^sub>n\<B>\<O>\<S>\<S>: "((X).boss) \<tau> = ((\<lambda>_. X \<tau>).boss) \<tau>" by simp
+lemma cp_dot\<^sub>P\<^sub>e\<^sub>r\<^sub>s\<^sub>o\<^sub>n\<S>\<A>\<L>\<A>\<R>\<Y>: "((X).salary) \<tau> = ((\<lambda>_. X \<tau>).salary) \<tau>" by simp
+
+lemma cp_dot\<^sub>O\<^sub>c\<^sub>l\<^sub>A\<^sub>n\<^sub>y\<A>\<N>\<Y>_at_pre: "((X).any@pre) \<tau> = ((\<lambda>_. X \<tau>).any@pre) \<tau>" by simp
+lemma cp_dot\<^sub>P\<^sub>e\<^sub>r\<^sub>s\<^sub>o\<^sub>n\<B>\<O>\<S>\<S>_at_pre: "((X).boss@pre) \<tau> = ((\<lambda>_. X \<tau>).boss@pre) \<tau>" by simp
+lemma cp_dot\<^sub>P\<^sub>e\<^sub>r\<^sub>s\<^sub>o\<^sub>n\<S>\<A>\<L>\<A>\<R>\<Y>_at_pre: "((X).salary@pre) \<tau> = ((\<lambda>_. X \<tau>).salary@pre) \<tau>" by simp
 
 lemmas cp_dot\<^sub>O\<^sub>c\<^sub>l\<^sub>A\<^sub>n\<^sub>y\<A>\<N>\<Y>_I [simp, intro!]=
        cp_dot\<^sub>O\<^sub>c\<^sub>l\<^sub>A\<^sub>n\<^sub>y\<A>\<N>\<Y>[THEN allI[THEN allI],
@@ -851,33 +860,33 @@ lemmas cp_dot\<^sub>P\<^sub>e\<^sub>r\<^sub>s\<^sub>o\<^sub>n\<S>\<A>\<L>\<A>\<R
 subsection{* Execution with invalid or null as argument *}
 
 lemma dot\<^sub>O\<^sub>c\<^sub>l\<^sub>A\<^sub>n\<^sub>y\<A>\<N>\<Y>_nullstrict [simp]: "(null).any = invalid"
-by(rule ext, simp add: null_fun_def null_option_def bot_option_def null_def invalid_def eval_extract_def)
+by(rule ext, simp add: null_fun_def null_option_def bot_option_def null_def invalid_def)
 lemma dot\<^sub>O\<^sub>c\<^sub>l\<^sub>A\<^sub>n\<^sub>y\<A>\<N>\<Y>_at_pre_nullstrict [simp] : "(null).any@pre = invalid"
-by(rule ext, simp add: null_fun_def null_option_def bot_option_def null_def invalid_def eval_extract_def)
+by(rule ext, simp add: null_fun_def null_option_def bot_option_def null_def invalid_def)
 lemma dot\<^sub>O\<^sub>c\<^sub>l\<^sub>A\<^sub>n\<^sub>y\<A>\<N>\<Y>_strict [simp] : "(invalid).any = invalid"
-by(rule ext, simp add: null_fun_def null_option_def bot_option_def null_def invalid_def eval_extract_def)
+by(rule ext, simp add: null_fun_def null_option_def bot_option_def null_def invalid_def)
 lemma dot\<^sub>O\<^sub>c\<^sub>l\<^sub>A\<^sub>n\<^sub>y\<A>\<N>\<Y>_at_pre_strict [simp] : "(invalid).any@pre = invalid"
-by(rule ext, simp add: null_fun_def null_option_def bot_option_def null_def invalid_def eval_extract_def)
+by(rule ext, simp add: null_fun_def null_option_def bot_option_def null_def invalid_def)
 
 
 lemma dot\<^sub>P\<^sub>e\<^sub>r\<^sub>s\<^sub>o\<^sub>n\<B>\<O>\<S>\<S>_nullstrict [simp]: "(null).boss = invalid"
-by(rule ext, simp add: null_fun_def null_option_def bot_option_def null_def invalid_def eval_extract_def)
+by(rule ext, simp add: null_fun_def null_option_def bot_option_def null_def invalid_def)
 lemma dot\<^sub>P\<^sub>e\<^sub>r\<^sub>s\<^sub>o\<^sub>n\<B>\<O>\<S>\<S>_at_pre_nullstrict [simp] : "(null).boss@pre = invalid"
-by(rule ext, simp add: null_fun_def null_option_def bot_option_def null_def invalid_def eval_extract_def)
+by(rule ext, simp add: null_fun_def null_option_def bot_option_def null_def invalid_def)
 lemma dot\<^sub>P\<^sub>e\<^sub>r\<^sub>s\<^sub>o\<^sub>n\<B>\<O>\<S>\<S>_strict [simp] : "(invalid).boss = invalid"
-by(rule ext, simp add: null_fun_def null_option_def bot_option_def null_def invalid_def eval_extract_def)
+by(rule ext, simp add: null_fun_def null_option_def bot_option_def null_def invalid_def)
 lemma dot\<^sub>P\<^sub>e\<^sub>r\<^sub>s\<^sub>o\<^sub>n\<B>\<O>\<S>\<S>_at_pre_strict [simp] : "(invalid).boss@pre = invalid"
-by(rule ext, simp add: null_fun_def null_option_def bot_option_def null_def invalid_def eval_extract_def)
+by(rule ext, simp add: null_fun_def null_option_def bot_option_def null_def invalid_def)
 
 
 lemma dot\<^sub>P\<^sub>e\<^sub>r\<^sub>s\<^sub>o\<^sub>n\<S>\<A>\<L>\<A>\<R>\<Y>_nullstrict [simp]: "(null).salary = invalid"
-by(rule ext, simp add: null_fun_def null_option_def bot_option_def null_def invalid_def eval_extract_def)
+by(rule ext, simp add: null_fun_def null_option_def bot_option_def null_def invalid_def)
 lemma dot\<^sub>P\<^sub>e\<^sub>r\<^sub>s\<^sub>o\<^sub>n\<S>\<A>\<L>\<A>\<R>\<Y>_at_pre_nullstrict [simp] : "(null).salary@pre = invalid"
-by(rule ext, simp add: null_fun_def null_option_def bot_option_def null_def invalid_def eval_extract_def)
+by(rule ext, simp add: null_fun_def null_option_def bot_option_def null_def invalid_def)
 lemma dot\<^sub>P\<^sub>e\<^sub>r\<^sub>s\<^sub>o\<^sub>n\<S>\<A>\<L>\<A>\<R>\<Y>_strict [simp] : "(invalid).salary = invalid"
-by(rule ext, simp add: null_fun_def null_option_def bot_option_def null_def invalid_def eval_extract_def)
+by(rule ext, simp add: null_fun_def null_option_def bot_option_def null_def invalid_def)
 lemma dot\<^sub>P\<^sub>e\<^sub>r\<^sub>s\<^sub>o\<^sub>n\<S>\<A>\<L>\<A>\<R>\<Y>_at_pre_strict [simp] : "(invalid).salary@pre = invalid"
-by(rule ext, simp add: null_fun_def null_option_def bot_option_def null_def invalid_def eval_extract_def)
+by(rule ext, simp add: null_fun_def null_option_def bot_option_def null_def invalid_def)
 
 
 section{* A little infra-structure on example states.*}
@@ -954,7 +963,8 @@ lemma basic_\<tau>_wff: "WFF(\<sigma>\<^sub>1,\<sigma>\<^sub>1')"
 by(auto simp: WFF_def \<sigma>\<^sub>1_def \<sigma>\<^sub>1'_def
               oid0_def oid1_def oid2_def oid3_def oid4_def oid5_def oid6_def oid7_def oid8_def
               oid_of_\<AA>_def oid_of_type\<^sub>P\<^sub>e\<^sub>r\<^sub>s\<^sub>o\<^sub>n_def oid_of_type\<^sub>O\<^sub>c\<^sub>l\<^sub>A\<^sub>n\<^sub>y_def
-              person1_def person2_def person3_def person4_def person5_def person6_def person7_def person8_def person9_def)
+              person1_def person2_def person3_def person4_def
+              person5_def person6_def person7_def person8_def person9_def)
 
 lemma [simp,code_unfold]: "dom (heap \<sigma>\<^sub>1) = {oid0,oid1,(*,oid2*)oid3,oid4,oid5(*,oid6,oid7*),oid8}"
 by(auto simp: \<sigma>\<^sub>1_def)
@@ -1096,7 +1106,8 @@ by(simp add: OclValid_def OclIsMaintained_def
 (* (* access to an oclany object not yet supported *) value "  (\<sigma>\<^sub>1,\<sigma>\<^sub>1') \<Turnstile>     ((X\<^sub>P\<^sub>e\<^sub>r\<^sub>s\<^sub>o\<^sub>n7 .oclAsType(Person) .boss .salary)   \<doteq> \<three>\<two>\<zero>\<zero> )" *)
 value "\<And>s\<^sub>p\<^sub>r\<^sub>e s\<^sub>p\<^sub>o\<^sub>s\<^sub>t.   (s\<^sub>p\<^sub>r\<^sub>e,s\<^sub>p\<^sub>o\<^sub>s\<^sub>t) \<Turnstile>     \<upsilon>(X\<^sub>P\<^sub>e\<^sub>r\<^sub>s\<^sub>o\<^sub>n7 .oclAsType(Person))"
 value "\<And>    s\<^sub>p\<^sub>o\<^sub>s\<^sub>t.    (\<sigma>\<^sub>1,s\<^sub>p\<^sub>o\<^sub>s\<^sub>t) \<Turnstile> not(\<upsilon>(X\<^sub>P\<^sub>e\<^sub>r\<^sub>s\<^sub>o\<^sub>n7 .oclAsType(Person) .boss@pre))"
-lemma "\<And>s\<^sub>p\<^sub>r\<^sub>e s\<^sub>p\<^sub>o\<^sub>s\<^sub>t.   (s\<^sub>p\<^sub>r\<^sub>e,s\<^sub>p\<^sub>o\<^sub>s\<^sub>t) \<Turnstile>     ((X\<^sub>P\<^sub>e\<^sub>r\<^sub>s\<^sub>o\<^sub>n7 .oclAsType(Person) .oclAsType(OclAny) .oclAsType(Person))
+lemma "\<And>s\<^sub>p\<^sub>r\<^sub>e s\<^sub>p\<^sub>o\<^sub>s\<^sub>t.   (s\<^sub>p\<^sub>r\<^sub>e,s\<^sub>p\<^sub>o\<^sub>s\<^sub>t) \<Turnstile>     ((X\<^sub>P\<^sub>e\<^sub>r\<^sub>s\<^sub>o\<^sub>n7 .oclAsType(Person) .oclAsType(OclAny)
+                                                                   .oclAsType(Person))
                                       \<doteq> (X\<^sub>P\<^sub>e\<^sub>r\<^sub>s\<^sub>o\<^sub>n7 .oclAsType(Person)))"
 by(rule up_down_cast_Person_OclAny_Person', simp add: X\<^sub>P\<^sub>e\<^sub>r\<^sub>s\<^sub>o\<^sub>n7_def OclValid_def valid_def person7_def)
 lemma "               (\<sigma>\<^sub>1,\<sigma>\<^sub>1') \<Turnstile>       (X\<^sub>P\<^sub>e\<^sub>r\<^sub>s\<^sub>o\<^sub>n7 .oclIsNew())"
@@ -1126,8 +1137,10 @@ lemma \<sigma>_modifiedonly: "(\<sigma>\<^sub>1,\<sigma>\<^sub>1') \<Turnstile> 
                     (*, X\<^sub>P\<^sub>e\<^sub>r\<^sub>s\<^sub>o\<^sub>n9 .oclAsType(OclAny)*)}->oclIsModifiedOnly())"
  apply(simp add: OclIsModifiedOnly_def OclValid_def
                  oid0_def oid1_def oid2_def oid3_def oid4_def oid5_def oid6_def oid7_def oid8_def
-                 X\<^sub>P\<^sub>e\<^sub>r\<^sub>s\<^sub>o\<^sub>n1_def X\<^sub>P\<^sub>e\<^sub>r\<^sub>s\<^sub>o\<^sub>n2_def X\<^sub>P\<^sub>e\<^sub>r\<^sub>s\<^sub>o\<^sub>n3_def X\<^sub>P\<^sub>e\<^sub>r\<^sub>s\<^sub>o\<^sub>n4_def X\<^sub>P\<^sub>e\<^sub>r\<^sub>s\<^sub>o\<^sub>n5_def X\<^sub>P\<^sub>e\<^sub>r\<^sub>s\<^sub>o\<^sub>n6_def X\<^sub>P\<^sub>e\<^sub>r\<^sub>s\<^sub>o\<^sub>n7_def X\<^sub>P\<^sub>e\<^sub>r\<^sub>s\<^sub>o\<^sub>n8_def X\<^sub>P\<^sub>e\<^sub>r\<^sub>s\<^sub>o\<^sub>n9_def
-                 person1_def person2_def person3_def person4_def person5_def person6_def person7_def person8_def person9_def
+                 X\<^sub>P\<^sub>e\<^sub>r\<^sub>s\<^sub>o\<^sub>n1_def X\<^sub>P\<^sub>e\<^sub>r\<^sub>s\<^sub>o\<^sub>n2_def X\<^sub>P\<^sub>e\<^sub>r\<^sub>s\<^sub>o\<^sub>n3_def X\<^sub>P\<^sub>e\<^sub>r\<^sub>s\<^sub>o\<^sub>n4_def
+                 X\<^sub>P\<^sub>e\<^sub>r\<^sub>s\<^sub>o\<^sub>n5_def X\<^sub>P\<^sub>e\<^sub>r\<^sub>s\<^sub>o\<^sub>n6_def X\<^sub>P\<^sub>e\<^sub>r\<^sub>s\<^sub>o\<^sub>n7_def X\<^sub>P\<^sub>e\<^sub>r\<^sub>s\<^sub>o\<^sub>n8_def X\<^sub>P\<^sub>e\<^sub>r\<^sub>s\<^sub>o\<^sub>n9_def
+                 person1_def person2_def person3_def person4_def
+                 person5_def person6_def person7_def person8_def person9_def
                  image_def)
  apply(simp add: OclIncluding_rep_set mtSet_rep_set null_option_def bot_option_def)
  apply(simp add: oid_of_option_def oid_of_type\<^sub>O\<^sub>c\<^sub>l\<^sub>A\<^sub>n\<^sub>y_def, clarsimp)
@@ -1152,9 +1165,12 @@ proof -
   apply(subst abs_rep_simp'[symmetric], simp)
  by(simp add: OclIncluding_rep_set mtSet_rep_set)
 
- have excluding1: "\<And>S a b c d e \<tau>. (\<lambda>_. Abs_Set_0 \<lfloor>\<lfloor> {\<lfloor>\<lfloor>a\<rfloor>\<rfloor>, \<lfloor>\<lfloor>b\<rfloor>\<rfloor>, \<lfloor>\<lfloor>c\<rfloor>\<rfloor>, \<lfloor>\<lfloor>d\<rfloor>\<rfloor>} \<rfloor>\<rfloor>)->excluding(\<lambda>\<tau>. \<lfloor>\<lfloor>e\<rfloor>\<rfloor>) \<tau> = Abs_Set_0 \<lfloor>\<lfloor> {\<lfloor>\<lfloor>a\<rfloor>\<rfloor>, \<lfloor>\<lfloor>b\<rfloor>\<rfloor>, \<lfloor>\<lfloor>c\<rfloor>\<rfloor>, \<lfloor>\<lfloor>d\<rfloor>\<rfloor>} - {\<lfloor>\<lfloor>e\<rfloor>\<rfloor>} \<rfloor>\<rfloor>"
+ have excluding1: "\<And>S a b c d e \<tau>.
+                   (\<lambda>_. Abs_Set_0 \<lfloor>\<lfloor> {\<lfloor>\<lfloor>a\<rfloor>\<rfloor>, \<lfloor>\<lfloor>b\<rfloor>\<rfloor>, \<lfloor>\<lfloor>c\<rfloor>\<rfloor>, \<lfloor>\<lfloor>d\<rfloor>\<rfloor>} \<rfloor>\<rfloor>)->excluding(\<lambda>\<tau>. \<lfloor>\<lfloor>e\<rfloor>\<rfloor>) \<tau> =
+                   Abs_Set_0 \<lfloor>\<lfloor> {\<lfloor>\<lfloor>a\<rfloor>\<rfloor>, \<lfloor>\<lfloor>b\<rfloor>\<rfloor>, \<lfloor>\<lfloor>c\<rfloor>\<rfloor>, \<lfloor>\<lfloor>d\<rfloor>\<rfloor>} - {\<lfloor>\<lfloor>e\<rfloor>\<rfloor>} \<rfloor>\<rfloor>"
   apply(simp add: OclExcluding_def)
-  apply(simp add: defined_def OclValid_def bot_fun_def bot_Set_0_def null_fun_def  null_Set_0_def false_def true_def)
+  apply(simp add: defined_def OclValid_def false_def true_def
+                  bot_fun_def bot_Set_0_def null_fun_def null_Set_0_def)
   apply(rule conjI)
    apply(rule impI, subst (asm) Abs_Set_0_inject) apply( simp add: bot_option_def)+
   apply(rule conjI)
@@ -1174,17 +1190,22 @@ proof -
                      (*, X\<^sub>P\<^sub>e\<^sub>r\<^sub>s\<^sub>o\<^sub>n9 .oclAsType(OclAny)*)}"])
    apply(cut_tac \<sigma>_modifiedonly)
    apply(simp only: OclValid_def
-                   X\<^sub>P\<^sub>e\<^sub>r\<^sub>s\<^sub>o\<^sub>n1_def X\<^sub>P\<^sub>e\<^sub>r\<^sub>s\<^sub>o\<^sub>n2_def X\<^sub>P\<^sub>e\<^sub>r\<^sub>s\<^sub>o\<^sub>n3_def X\<^sub>P\<^sub>e\<^sub>r\<^sub>s\<^sub>o\<^sub>n4_def X\<^sub>P\<^sub>e\<^sub>r\<^sub>s\<^sub>o\<^sub>n5_def X\<^sub>P\<^sub>e\<^sub>r\<^sub>s\<^sub>o\<^sub>n6_def X\<^sub>P\<^sub>e\<^sub>r\<^sub>s\<^sub>o\<^sub>n7_def X\<^sub>P\<^sub>e\<^sub>r\<^sub>s\<^sub>o\<^sub>n8_def X\<^sub>P\<^sub>e\<^sub>r\<^sub>s\<^sub>o\<^sub>n9_def
-                    person1_def person2_def person3_def person4_def person5_def person6_def person7_def person8_def person9_def
+                    X\<^sub>P\<^sub>e\<^sub>r\<^sub>s\<^sub>o\<^sub>n1_def X\<^sub>P\<^sub>e\<^sub>r\<^sub>s\<^sub>o\<^sub>n2_def X\<^sub>P\<^sub>e\<^sub>r\<^sub>s\<^sub>o\<^sub>n3_def X\<^sub>P\<^sub>e\<^sub>r\<^sub>s\<^sub>o\<^sub>n4_def
+                    X\<^sub>P\<^sub>e\<^sub>r\<^sub>s\<^sub>o\<^sub>n5_def X\<^sub>P\<^sub>e\<^sub>r\<^sub>s\<^sub>o\<^sub>n6_def X\<^sub>P\<^sub>e\<^sub>r\<^sub>s\<^sub>o\<^sub>n7_def X\<^sub>P\<^sub>e\<^sub>r\<^sub>s\<^sub>o\<^sub>n8_def X\<^sub>P\<^sub>e\<^sub>r\<^sub>s\<^sub>o\<^sub>n9_def
+                    person1_def person2_def person3_def person4_def
+                    person5_def person6_def person7_def person8_def person9_def
                     OclAsType\<^sub>O\<^sub>c\<^sub>l\<^sub>A\<^sub>n\<^sub>y_Person)
    apply(subst cp_OclIsModifiedOnly, subst cp_OclExcluding,
      subst (asm) cp_OclIsModifiedOnly, simp add: including4 excluding1)
 
-  apply(simp only: X\<^sub>P\<^sub>e\<^sub>r\<^sub>s\<^sub>o\<^sub>n1_def X\<^sub>P\<^sub>e\<^sub>r\<^sub>s\<^sub>o\<^sub>n2_def X\<^sub>P\<^sub>e\<^sub>r\<^sub>s\<^sub>o\<^sub>n3_def X\<^sub>P\<^sub>e\<^sub>r\<^sub>s\<^sub>o\<^sub>n4_def X\<^sub>P\<^sub>e\<^sub>r\<^sub>s\<^sub>o\<^sub>n5_def X\<^sub>P\<^sub>e\<^sub>r\<^sub>s\<^sub>o\<^sub>n6_def X\<^sub>P\<^sub>e\<^sub>r\<^sub>s\<^sub>o\<^sub>n7_def X\<^sub>P\<^sub>e\<^sub>r\<^sub>s\<^sub>o\<^sub>n8_def X\<^sub>P\<^sub>e\<^sub>r\<^sub>s\<^sub>o\<^sub>n9_def
-                   person1_def person2_def person3_def person4_def person5_def person6_def person7_def person8_def person9_def)
+  apply(simp only: X\<^sub>P\<^sub>e\<^sub>r\<^sub>s\<^sub>o\<^sub>n1_def X\<^sub>P\<^sub>e\<^sub>r\<^sub>s\<^sub>o\<^sub>n2_def X\<^sub>P\<^sub>e\<^sub>r\<^sub>s\<^sub>o\<^sub>n3_def X\<^sub>P\<^sub>e\<^sub>r\<^sub>s\<^sub>o\<^sub>n4_def
+                   X\<^sub>P\<^sub>e\<^sub>r\<^sub>s\<^sub>o\<^sub>n5_def X\<^sub>P\<^sub>e\<^sub>r\<^sub>s\<^sub>o\<^sub>n6_def X\<^sub>P\<^sub>e\<^sub>r\<^sub>s\<^sub>o\<^sub>n7_def X\<^sub>P\<^sub>e\<^sub>r\<^sub>s\<^sub>o\<^sub>n8_def X\<^sub>P\<^sub>e\<^sub>r\<^sub>s\<^sub>o\<^sub>n9_def
+                   person1_def person2_def person3_def person4_def
+                   person5_def person6_def person7_def person8_def person9_def)
   apply(simp add: OclIncluding_rep_set mtSet_rep_set
                   oid0_def oid1_def oid2_def oid3_def oid4_def oid5_def oid6_def oid7_def oid8_def)
-  apply(simp add: StrictRefEq\<^sub>O\<^sub>b\<^sub>j\<^sub>e\<^sub>c\<^sub>t_def null_option_def bot_option_def oid_of_option_def oid_of_type\<^sub>O\<^sub>c\<^sub>l\<^sub>A\<^sub>n\<^sub>y_def OclNot_def OclValid_def)
+  apply(simp add: StrictRefEq\<^sub>O\<^sub>b\<^sub>j\<^sub>e\<^sub>c\<^sub>t_def oid_of_option_def oid_of_type\<^sub>O\<^sub>c\<^sub>l\<^sub>A\<^sub>n\<^sub>y_def OclNot_def OclValid_def
+                  null_option_def bot_option_def)
  done
 qed
 
@@ -1215,9 +1236,12 @@ proof -
  by(simp)
 qed
 
-lemma "\<And>\<sigma>\<^sub>1.    (\<sigma>\<^sub>1,\<sigma>\<^sub>1') \<Turnstile>      (Person .allInstances() \<doteq> Set{ X\<^sub>P\<^sub>e\<^sub>r\<^sub>s\<^sub>o\<^sub>n1, X\<^sub>P\<^sub>e\<^sub>r\<^sub>s\<^sub>o\<^sub>n2, X\<^sub>P\<^sub>e\<^sub>r\<^sub>s\<^sub>o\<^sub>n3, X\<^sub>P\<^sub>e\<^sub>r\<^sub>s\<^sub>o\<^sub>n4(*, X\<^sub>P\<^sub>e\<^sub>r\<^sub>s\<^sub>o\<^sub>n5*), X\<^sub>P\<^sub>e\<^sub>r\<^sub>s\<^sub>o\<^sub>n6, X\<^sub>P\<^sub>e\<^sub>r\<^sub>s\<^sub>o\<^sub>n7 .oclAsType(Person)(*, X\<^sub>P\<^sub>e\<^sub>r\<^sub>s\<^sub>o\<^sub>n8*), X\<^sub>P\<^sub>e\<^sub>r\<^sub>s\<^sub>o\<^sub>n9 })"
+lemma "\<And>\<sigma>\<^sub>1.
+ (\<sigma>\<^sub>1,\<sigma>\<^sub>1') \<Turnstile> (Person .allInstances() \<doteq> Set{ X\<^sub>P\<^sub>e\<^sub>r\<^sub>s\<^sub>o\<^sub>n1, X\<^sub>P\<^sub>e\<^sub>r\<^sub>s\<^sub>o\<^sub>n2, X\<^sub>P\<^sub>e\<^sub>r\<^sub>s\<^sub>o\<^sub>n3, X\<^sub>P\<^sub>e\<^sub>r\<^sub>s\<^sub>o\<^sub>n4(*, X\<^sub>P\<^sub>e\<^sub>r\<^sub>s\<^sub>o\<^sub>n5*), X\<^sub>P\<^sub>e\<^sub>r\<^sub>s\<^sub>o\<^sub>n6,
+                                           X\<^sub>P\<^sub>e\<^sub>r\<^sub>s\<^sub>o\<^sub>n7 .oclAsType(Person)(*, X\<^sub>P\<^sub>e\<^sub>r\<^sub>s\<^sub>o\<^sub>n8*), X\<^sub>P\<^sub>e\<^sub>r\<^sub>s\<^sub>o\<^sub>n9 })"
 proof -
- def p7 \<equiv> "((((\<lambda>_. \<lfloor>\<lfloor>mk\<^sub>O\<^sub>c\<^sub>l\<^sub>A\<^sub>n\<^sub>y 6 \<lfloor>(\<lfloor>3200\<rfloor>, \<lfloor>6\<rfloor>)\<rfloor>\<rfloor>\<rfloor>) :: \<AA> state \<times> \<AA> state \<Rightarrow> type\<^sub>O\<^sub>c\<^sub>l\<^sub>A\<^sub>n\<^sub>y option option) .oclAsType(Person)))"
+ def p7 \<equiv> "((((\<lambda>_. \<lfloor>\<lfloor>mk\<^sub>O\<^sub>c\<^sub>l\<^sub>A\<^sub>n\<^sub>y 6 \<lfloor>(\<lfloor>3200\<rfloor>, \<lfloor>6\<rfloor>)\<rfloor>\<rfloor>\<rfloor>)
+                :: \<AA> state \<times> \<AA> state \<Rightarrow> type\<^sub>O\<^sub>c\<^sub>l\<^sub>A\<^sub>n\<^sub>y option option) .oclAsType(Person)))"
 
  have incl_cp_all : "\<And>S a.
                      \<forall>X \<tau> \<tau>'. X \<tau> = X \<tau>' \<longrightarrow>
@@ -1273,7 +1297,8 @@ proof -
   apply(rule incl_cp_all[OF cp_2], (simp add: p7_def)+)
  by(intro allI, (rule OclIncluding_cp_all, simp_all add: mtSet_cp_all)+)
 
- have including_subst_set : "\<And>(s::('\<AA>,'a::null)Set) t x y \<tau>. \<tau> \<Turnstile> \<delta> t \<Longrightarrow> \<tau> \<Turnstile> \<upsilon> y \<Longrightarrow> \<tau> \<Turnstile> s \<doteq> t \<Longrightarrow> x = y \<Longrightarrow> \<tau> \<Turnstile> s->including(x) \<doteq> (t->including(y))"
+ have including_subst_set : "\<And>(s::('\<AA>,'a::null)Set) t x y \<tau>. \<tau> \<Turnstile> \<delta> t \<Longrightarrow> \<tau> \<Turnstile> \<upsilon> y \<Longrightarrow>
+                             \<tau> \<Turnstile> s \<doteq> t \<Longrightarrow> x = y \<Longrightarrow> \<tau> \<Turnstile> s->including(x) \<doteq> (t->including(y))"
   apply(simp only:)
   apply(rule including_subst_set', simp_all only:)
  by(auto simp: OclValid_def OclIf_def invalid_def bot_option_def OclNot_def split : split_if_asm)
@@ -1281,7 +1306,8 @@ proof -
  show "\<And>\<sigma>\<^sub>1. ?thesis \<sigma>\<^sub>1"
   apply(subst perm_\<sigma>\<^sub>1')
   apply(simp only: oid0_def oid1_def oid2_def oid3_def oid4_def oid5_def oid6_def oid7_def oid8_def
-                   X\<^sub>P\<^sub>e\<^sub>r\<^sub>s\<^sub>o\<^sub>n1_def X\<^sub>P\<^sub>e\<^sub>r\<^sub>s\<^sub>o\<^sub>n2_def X\<^sub>P\<^sub>e\<^sub>r\<^sub>s\<^sub>o\<^sub>n3_def X\<^sub>P\<^sub>e\<^sub>r\<^sub>s\<^sub>o\<^sub>n4_def X\<^sub>P\<^sub>e\<^sub>r\<^sub>s\<^sub>o\<^sub>n5_def X\<^sub>P\<^sub>e\<^sub>r\<^sub>s\<^sub>o\<^sub>n6_def X\<^sub>P\<^sub>e\<^sub>r\<^sub>s\<^sub>o\<^sub>n7_def X\<^sub>P\<^sub>e\<^sub>r\<^sub>s\<^sub>o\<^sub>n8_def X\<^sub>P\<^sub>e\<^sub>r\<^sub>s\<^sub>o\<^sub>n9_def
+                   X\<^sub>P\<^sub>e\<^sub>r\<^sub>s\<^sub>o\<^sub>n1_def X\<^sub>P\<^sub>e\<^sub>r\<^sub>s\<^sub>o\<^sub>n2_def X\<^sub>P\<^sub>e\<^sub>r\<^sub>s\<^sub>o\<^sub>n3_def X\<^sub>P\<^sub>e\<^sub>r\<^sub>s\<^sub>o\<^sub>n4_def
+                   X\<^sub>P\<^sub>e\<^sub>r\<^sub>s\<^sub>o\<^sub>n5_def X\<^sub>P\<^sub>e\<^sub>r\<^sub>s\<^sub>o\<^sub>n6_def X\<^sub>P\<^sub>e\<^sub>r\<^sub>s\<^sub>o\<^sub>n7_def X\<^sub>P\<^sub>e\<^sub>r\<^sub>s\<^sub>o\<^sub>n8_def X\<^sub>P\<^sub>e\<^sub>r\<^sub>s\<^sub>o\<^sub>n9_def
                    person7_def)
   apply(subst state_update_vs_allInstances_at_post_tc, simp, simp add: OclAsType\<^sub>P\<^sub>e\<^sub>r\<^sub>s\<^sub>o\<^sub>n_\<AA>_def, simp, rule cp_1[simplified p7_def], rule including_subst_set, simp, simp)
    apply(subst state_update_vs_allInstances_at_post_tc, simp, simp add: OclAsType\<^sub>P\<^sub>e\<^sub>r\<^sub>s\<^sub>o\<^sub>n_\<AA>_def, simp, rule cp_2[simplified p7_def], rule including_subst_set, simp, simp)
